src/lib/extraction/Bit.ml
@@ -74,6 +74,73 @@ module Three =
              | BU -> BU)
     | BU -> BU
 
+  (** val bit_add : ubit -> ubit -> ubit * ubit **)
+
+  let bit_add lhs rhs =
+    match lhs with
+    | B0 -> (match rhs with
+             | B0 -> (B0, B0)
+             | x -> (x, B0))
+    | B1 -> (match rhs with
+             | B0 -> (B1, B0)
+             | B1 -> (B0, B1)
+             | BU -> (BU, BU))
+    | BU -> (match rhs with
+             | B0 -> (BU, B0)
+             | _ -> (BU, BU))
+
+  (** val bit_add_carry : ubit -> ubit -> ubit -> ubit * ubit **)
+
+  let bit_add_carry lhs rhs carry =
+    let p = (lhs, rhs) in
+    let (u0, u1) = p in
+    (match u0 with
+     | B0 ->
+       (match u1 with
+        | B0 -> (match carry with
+                 | B0 -> (B0, B0)
+                 | x -> (x, B0))
+        | B1 ->
+          (match carry with
+           | B0 -> (B1, B0)
+           | B1 -> (B0, B1)
+           | BU -> (BU, BU))
+        | BU -> (match carry with
+                 | B0 -> (BU, B0)
+                 | _ -> (BU, BU)))
+     | B1 ->
+       (match u1 with
+        | B0 ->
+          (match carry with
+           | B0 -> (B1, B0)
+           | B1 -> (B0, B1)
+           | BU -> (BU, BU))
+        | B1 -> (match carry with
+                 | B0 -> (B0, B1)
+                 | x -> (x, x))
+        | BU -> (BU, BU))
+     | BU ->
+       (match u1 with
+        | B0 -> (match carry with
+                 | B0 -> (BU, B0)
+                 | _ -> (BU, BU))
+        | _ -> (BU, BU)))
+
+  (** val bitlist_add_carry_acc :
+      ubit list -> ubit list -> ubit -> ubit list -> ubit list * ubit **)
+
+  let rec bitlist_add_carry_acc xs ys c zs =
+    match xs with
+    | [] -> (zs, c)
+    | x :: xs0 ->
+      (match ys with
+       | [] ->
+         let (z, c0) = bit_add x c in
+         bitlist_add_carry_acc xs0 ys c0 (z :: zs)
+       | y :: ys0 ->
+         let (z, c0) = bit_add_carry x y c in
+         bitlist_add_carry_acc xs0 ys0 c0 (z :: zs))
+
   (** val bit_join : ubit -> ubit -> ubit **)
 
   let bit_join x y =
